Fix incorrect naming of Curve25519 top-level function

code/curve25519/Hacl.Curve25519_64.fst
@@ -9,21 +9,22 @@ open Lib.Buffer
 open Hacl.Impl.Curve25519.Fields
 open Hacl.Impl.Curve25519.Generic
 
-module S = Spec.Curve25519
+
 
 val secret_to_public:
     pub:lbuffer uint8 32ul
-  -> priv:lbuffer uint8 32ul
-  -> Stack unit
+  -> priv:lbuffer uint8 32ul ->
+  Stack unit
     (requires fun h0 ->
       live h0 pub /\ live h0 priv /\ disjoint pub priv)
     (ensures  fun h0 _ h1 -> modifies (loc pub) h0 h1 /\
-      as_seq h1 pub == S.secret_to_public (as_seq h0 priv))
+      as_seq h1 pub == Spec.Curve25519.secret_to_public (as_seq h0 priv))
+
 let secret_to_public pub priv =
   secret_to_public #M64 pub priv
 
 
-val ecdh:
+val scalarmult:
     shared:lbuffer uint8 32ul
   -> my_priv:lbuffer uint8 32ul
   -> their_pub:lbuffer uint8 32ul
@@ -32,6 +33,7 @@ val ecdh:
       live h0 shared /\ live h0 my_priv /\ live h0 their_pub /\
       disjoint shared my_priv /\ disjoint shared their_pub)
     (ensures  fun h0 _ h1 -> modifies (loc shared) h0 h1 /\
-      as_seq h1 shared == S.scalarmult (as_seq h0 my_priv) (as_seq h0 their_pub))
-let ecdh shared my_priv their_pub =
+      as_seq h1 shared == Spec.Curve25519.scalarmult (as_seq h0 my_priv) (as_seq h0 their_pub))
+
+let scalarmult shared my_priv their_pub =
   scalarmult #M64 shared my_priv their_pub
